theories/Types/TSyms.v
@@ -1,31 +1,33 @@
-Require Import MirrorCore.Types.ModularTypes.
+Require Import MirrorCore.Types.ModularTypesT.
 
 Section sum.
-  Variable T U : nat -> Set.
-  Inductive tsym_sum (n : nat) : Set :=
+  Variable kind : Set.
+  Variable kindD : kind -> Type@{Ukind}.
+  Variable T U : kind -> Set.
+  Inductive tsym_sum (n : kind) : Set :=
   | TSym_left : T n -> tsym_sum n
   | TSym_right : U n -> tsym_sum n.
 
-  Variable TSym_T : TSym T.
-  Variable TSym_U : TSym U.
+  Variable TSym_T : TSym kindD T.
+  Variable TSym_U : TSym kindD U.
 
-  Instance TSym_sum : TSym tsym_sum :=
+  Instance TSym_sum : TSym kindD tsym_sum :=
   { symbolD := fun n x =>
-                 match x in tsym_sum _ return type_for_arity n with
-                 | TSym_left _ x => TSym_T.(@symbolD _) _ x
-                 | TSym_right _ x => TSym_U.(@symbolD _) _ x
+                 match x in tsym_sum _ return kindD n with
+                 | TSym_left _ x => TSym_T.(@symbolD _ _ _) _ x
+                 | TSym_right _ x => TSym_U.(@symbolD _ _ _) _ x
                  end
   ; symbol_dec := fun n x y =>
                     match x as x , y as y
                           return {x = y} + {x <> y}
                     with
                     | TSym_left _ x , TSym_left _ y =>
-                      match TSym_T.(@symbol_dec _) _ x y with
+                      match TSym_T.(@symbol_dec _ _ _) _ x y with
                       | left pf => left match pf with eq_refl => eq_refl end
                       | right pf => right (fun _ => _)
                       end
                     | TSym_right _ x , TSym_right _ y =>
-                      match TSym_U.(@symbol_dec _) _ x y with
+                      match TSym_U.(@symbol_dec _ _ _) _ x y with
                       | left pf => left match pf with eq_refl => eq_refl end
                       | right pf => right (fun _ => _)
                       end
