theories/Lambda/RewriteStrat.v
@@ -5,5 +5,5 @@ Require Export MirrorCore.Lambda.Rewrite.Repeat.
 Require Export MirrorCore.Lambda.Rewrite.Respectful.
 Require Export MirrorCore.Lambda.Rewrite.Reduce.
 Require Export MirrorCore.Lambda.Rewrite.Rewrite.
-Require Export MirrorCore.Lambda.Rewrite.HintDbs.
+(* Require Export MirrorCore.Lambda.Rewrite.HintDbsT. *)
 Require Export MirrorCore.Lambda.Rewrite.Tactic.
