theories/Types/FTypes.v
@@ -1,0 +1,414 @@
+(* Representation of first-order types *)
+Require Import ExtLib.Core.RelDec.
+Require Import ExtLib.Data.Vector.
+Require Import ExtLib.Data.SigT.
+Require Import ExtLib.Data.POption.
+Require Import ExtLib.Data.Positive.
+Require Import ExtLib.Tactics.
+Require Import ExtLib.Data.Eq.
+
+Require Import MirrorCore.Util.PolyAcc.
+Require Import MirrorCore.Util.PositivePolyMap.
+Require Import MirrorCore.TypesI.
+Require Import MirrorCore.Views.TypeView.
+
+Require Import MirrorCore.Types.ModularTypesT.
+
+Module TypeLang_mtyp <: TypeLang.
+  Definition kind := nat.
+  Definition Kstar := 0.
+  Definition kind_eq_dec (a b : kind) : {a = b} + {a <> b}.
+   decide equality.
+  Defined.
+
+  Fixpoint kindD (n : nat) : Type@{Ukind} :=
+    match n with
+    | 0 => Type@{Usmall}
+    | S n => Type@{Usmall} -> kindD n
+    end.
+
+  Fixpoint applyn' {n} (vs : vector Type@{Usmall} n)
+  : kindD n -> Type@{Usmall} :=
+    match vs in vector _ n return kindD n -> Type@{Usmall} with
+    | Vnil _ => fun T => T
+    | Vcons v vs => fun F => applyn' vs (F v)
+    end.
+  Definition applyn {n} (f : kindD n) (vs : vector Type@{Usmall} n)
+  : Type@{Usmall} :=
+    applyn' vs f.
+
+  Section with_symbols.
+
+    Variable symbol : kind -> Set.
+
+    Unset Elimination Schemes.
+
+    Inductive type' : kind -> Set :=
+    | tyArr : type' 0 -> type' 0 -> type' 0
+    | tyBase0 : symbol Kstar -> type' 0
+    | tyBase1 : symbol 1 -> type' 0 -> type' 0
+    | tyBase2 : symbol 2 -> type' 0 -> type' 0 -> type' 0
+    | tyApp : forall {n}, symbol (3 + n) -> vector (type' 0) (3 + n) -> type' 0
+    | tyProp : type' 0
+    | tyVar' : forall k, positive -> type' k. (** Reserved for unification, do not use **)
+
+    Definition tyVar := tyVar'.
+
+    Definition type := type'.
+
+    Section type_ind.
+      Variable P : type 0 -> Prop.
+      Hypotheses  (Harr : forall {a b}, P a -> P b -> P (tyArr a b))
+                  (Hbase0 : forall s, P (tyBase0 s))
+                  (Hbase1 : forall s {a}, P a -> P (tyBase1 s a))
+                  (Hbase2 : forall s {a b}, P a -> P b -> P (tyBase2 s a b))
+                  (Happ : forall {n} s ms, ForallV P ms -> P (@tyApp n s ms))
+                  (Hprop : P tyProp)
+                  (Hvar : forall p, P (tyVar' Kstar p)).
+      Fixpoint type_ind (x : type 0) : P x :=
+        match x as x in type' 0 return P x with
+        | tyArr a b => Harr _ _ (type_ind a) (type_ind b)
+        | tyBase0 s => Hbase0 s
+        | tyBase1 s a => Hbase1 s _ (type_ind a)
+        | tyBase2 s a b => Hbase2 s _ _ (type_ind a) (type_ind b)
+        | tyApp s ms =>
+          Happ _ s ms ((fix all {n} (ms : vector (type 0) n) : ForallV P ms :=
+                          match ms with
+                          | Vnil _ => ForallV_nil _
+                          | Vcons m ms => ForallV_cons _(type_ind m) (all ms)
+                          end) _ ms)
+        | tyProp => Hprop
+        | tyVar' 0 p => Hvar p
+        end.
+    End type_ind.
+
+    Variable ts : TSym kindD symbol.
+
+    Fixpoint default_type_for_kind n : kindD n :=
+      match n as n return kindD n with
+      | 0 => Empty_set
+      | S b => fun _ => default_type_for_kind b
+      end.
+
+
+    Fixpoint typeD {k} (t : type k) : kindD k :=
+      match t in type' k return kindD k with
+      | tyArr a b => typeD a -> typeD b
+      | tyBase0 s => symbolD kindD s
+      | tyBase1 s m => symbolD kindD s (typeD m)
+      | tyBase2 s m1 m2 => symbolD kindD s (typeD m1) (typeD m2)
+      | tyApp s ms => applyn (symbolD kindD s) (vector_map typeD ms)
+      | tyProp => Prop
+      | tyVar' n _ => default_type_for_kind n
+      end.
+
+    Inductive mtyp_acc (a : type Kstar) : type Kstar -> Prop :=
+    | tyAcc_tyArrL   : forall b, mtyp_acc a (tyArr a b)
+    | tyAcc_tyArrR   : forall b, mtyp_acc a (tyArr b a)
+    | tyAcc_tyBase1  : forall s, mtyp_acc a (tyBase1 s a)
+    | tyAcc_tyBase2L : forall s b, mtyp_acc a (tyBase2 s a b)
+    | tyAcc_tyBase2R : forall s b, mtyp_acc a (tyBase2 s b a)
+    | tyAcc_tyApp    : forall n s ms, vector_In a ms -> mtyp_acc a (@tyApp n s ms).
+
+
+    Theorem wf_mtyp_acc : well_founded mtyp_acc.
+    Proof.
+      red. eapply type_ind; constructor; inversion 1; subst; auto.
+      - apply inj_pair2 in H4.
+        subst. eapply ForallV_vector_In; eauto.
+    Defined.
+
+    Lemma Injective_tyArr : forall a b c d, tyArr a b = tyArr c d -> a = c /\ b = d.
+    Proof.
+      inversion 1; auto.
+    Defined.
+
+    Lemma Injective_tyBase0 : forall a b, tyBase0 a = tyBase0 b -> a = b.
+    Proof.
+      inversion 1; auto.
+    Defined.
+
+    Lemma Injective_tyBase1 : forall a b c d, tyBase1 a b = tyBase1 c d -> a = c /\ b = d.
+    Proof.
+      inversion 1; auto.
+    Defined.
+
+    Lemma Injective_tyBase2 : forall a b c d e f, tyBase2 a b c = tyBase2 d e f -> a = d /\ b = e /\ c = f.
+    Proof.
+      inversion 1; auto.
+    Defined.
+
+    Lemma Injective_tyApp : forall n a b c d, @tyApp n a b = @tyApp n c d -> a = c /\ b = d.
+    Proof.
+      intros.
+      refine
+        (match H in _ = Z
+               return match Z return Prop with
+                      | @tyApp N C D => forall pf : N = n,
+                          a = match pf with
+                              | eq_refl => C
+                              end /\ b = match pf with
+                                        | eq_refl => D
+                                        end
+                      | _ => True
+                      end
+         with
+         | eq_refl => _
+         end eq_refl).
+      intros. rewrite (UIP_refl pf). tauto.
+    Defined.
+
+    Fixpoint type_eq_dec {k} (a : type k) : forall b, {a = b} + {a <> b}.
+    refine
+      match a as a in type' k
+            return forall b : type k, {a = b} + {a <> b}
+      with
+      | tyArr l r => fun b =>
+        match b as b in type' z
+              return {match z as z return type' z -> Prop with
+                      | 0 => fun b => tyArr l r = b
+                      | _ => fun _ => False
+                      end b} + {match z as z return type' z -> Prop with
+                                | 0 => fun b => tyArr l r <> b
+                                | _ => fun _ => True
+                                end%type b}
+        with
+        | tyArr l' r' =>
+          match type_eq_dec _ l l' , type_eq_dec _ r r' with
+          | left pf , left pf' => left match pf , pf' with
+                                      | eq_refl , eq_refl => eq_refl
+                                      end
+          | _ , _ => right _
+          end
+        | _ => right _
+        end
+      | tyBase0 l => fun b =>
+        match b as b in type' z
+              return {match z as z return type' z -> Prop with
+                      | 0 => fun b => tyBase0 l = b
+                      | _ => fun _ => False
+                      end b} + {match z as z return type' z -> Prop with
+                                | 0 => fun b => tyBase0 l <> b
+                                | _ => fun _ => True
+                                end%type b}
+        with
+        | tyBase0 l' =>
+          match symbol_dec _ l l' with
+          | left pf => left _
+          | _ => right _
+          end
+        | _ => right _
+        end
+      | tyBase1 l r => fun b =>
+        match b as b in type' z
+              return {match z as z return type' z -> Prop with
+                      | 0 => fun b => tyBase1 l r = b
+                      | _ => fun _ => False
+                      end b} + {match z as z return type' z -> Prop with
+                                | 0 => fun b => tyBase1 l r <> b
+                                | _ => fun _ => True
+                                end%type b}
+        with
+        | tyBase1 l' r' =>
+          match symbol_dec _ l l' , type_eq_dec _ r r' with
+          | left pf , left pf' => left _
+          | _ , _ => right _
+          end
+        | _ => right _
+        end
+      | tyBase2 l r x => fun b =>
+        match b as b in type' z
+              return {match z as z return type' z -> Prop with
+                      | 0 => fun b => tyBase2 l r x = b
+                      | _ => fun _ => False
+                      end b} + {match z as z return type' z -> Prop with
+                                | 0 => fun b => tyBase2 l r x <> b
+                                | _ => fun _ => True
+                                end%type b}
+        with
+        | tyBase2 l' r' x' =>
+          match symbol_dec _ l l' , type_eq_dec _ r r' , type_eq_dec _ x x' with
+          | left pf , left pf' , left pf'' => left _
+          | _ , _ , _ => right _
+          end
+        | _ => right _
+        end
+      | @tyApp n s xs => fun b =>
+        match b as b in type' z
+              return {match z as z return type' z -> Prop with
+                      | 0 => fun b => tyApp s xs = b
+                      | _ => fun _ => False
+                      end b} + {match z as z return type' z -> Prop with
+                                | 0 => fun b => tyApp s xs <> b
+                                | _ => fun _ => True
+                                end%type b}
+        with
+        | @tyApp n' s' xs' =>
+          match PeanoNat.Nat.eq_dec n n' with
+          | left pf =>
+            match pf in _ = N
+                  return forall (s' : symbol (3+N)) (xs' : vector _ (3+N)),
+                           {@tyApp n s xs = @tyApp N s' xs'} +
+                           {@tyApp n s xs <> @tyApp N s' xs'}
+            with
+            | eq_refl => fun s' xs' =>
+              match symbol_dec _ s s' , vector_dec (@type_eq_dec Kstar) xs xs' with
+              | left pf , left pf' => left _
+              | _ , _ => right _
+              end
+            end s' xs'
+          | right _ => right _
+          end
+        | _ => right _
+        end
+      | tyProp => fun b =>
+        match b as b in type' z
+              return {match z as z return type' z -> Prop with
+                      | 0 => fun b => tyProp = b
+                      | _ => fun _ => False
+                      end b} + {match z as z return type' z -> Prop with
+                                | 0 => fun b => tyProp <> b
+                                | _ => fun _ => True
+                                end%type b}
+        with
+        | tyProp => left _
+        | _ => right _
+        end
+      | tyVar' _ n => fun b =>
+        match b as b in type' z
+              return {tyVar' _ n = b} + {tyVar' _ n <> b}
+        with
+        | tyVar' _ n' =>
+          match Pos.eq_dec n n' with
+          | left pf => left _
+          | _ => right _
+          end
+        | _ => right _
+        end
+      end.
+    all: try solve [ subst ; reflexivity
+                   | clear ; intro pf; inversion pf
+                   | intro pf ; inversion pf; auto
+                   | destruct k0; auto; inversion 1 ].
+    { intro. apply Injective_tyApp in H. tauto. }
+    { intro. apply Injective_tyApp in H. tauto. }
+    Defined.
+
+    Definition mtyp_cast (a b : type Kstar) : option (a = b) :=
+      match type_eq_dec a b with
+      | left pf => Some pf
+      | _ => None
+      end.
+
+    Instance RType_type : RType (type Kstar) :=
+    { typD := typeD
+    ; type_cast := mtyp_cast
+    ; tyAcc := mtyp_acc }.
+
+    Instance RTypeOk_type : RTypeOk.
+    refine
+      {| Relim_refl := fun _ _ _ => eq_refl
+       ; wf_tyAcc := wf_mtyp_acc
+       ; Relim_sym := ltac:(destruct pf; reflexivity)
+       ; Relim_trans := ltac:(destruct pf1; destruct pf2; reflexivity)
+       ; type_cast_refl := _
+       ; EquivDec_typ := type_eq_dec
+       |}.
+    simpl. unfold mtyp_cast. intros. rewrite dec_refl. reflexivity.
+    Defined.
+  End with_symbols.
+
+  Arguments tyBase0 {_} _.
+  Arguments tyBase1 {_} _ _.
+  Arguments tyBase2 {_} _ _ _.
+  Arguments tyApp {_ _} _ _.
+  Arguments tyArr {_} _ _.
+  Arguments tyProp {_}.
+  Arguments tyVar {_} _ _.
+  Arguments tyVar' {_} _ _.
+
+End TypeLang_mtyp.
+
+Module TypeLangUnify_mtyp <: TypeLangUnify with Module RT := TypeLang_mtyp.
+  Module RT := TypeLang_mtyp.
+  Import RT.
+
+  Section with_symbols.
+    Variable tsym : kind -> Set.
+
+    Definition Sub := pmap { k : kind & type tsym k }.
+    Definition add {n} (a :  positive) (b : type tsym n) (c : Sub)
+    : option Sub := Some (pmap_insert a c (@existT _ _ n b)).
+
+    Fixpoint type_unify {k} (a b : type tsym k) (s : Sub) {struct a}
+    : option Sub :=
+      match a with
+      | @tyArr _ da ca =>
+        match b with
+        | @tyArr _ db cb =>
+          match type_unify da db s with
+          | Some s' => type_unify ca cb s'
+          | _ => None
+          end
+        | @tyVar' _ _ v => add v a s
+        | _ => None
+        end
+      | @tyBase0 _ _ =>
+        match b with
+        | @tyBase0 _ _ => Some s
+        | @tyVar' _ _ v => add v a s
+        | _ => None
+        end
+      | @tyBase1 _ _ ta =>
+        match b with
+        | @tyBase1 _ _ tb => type_unify ta tb s
+        | @tyVar' _ _ v => add v a s
+        | _ => None
+        end
+      | @tyBase2 _ _ ta ta' =>
+        match b with
+        | @tyBase2 _ _ tb tb' =>
+          match type_unify ta tb s with
+          | Some s' => type_unify ta' tb' s'
+          | _ => None
+          end
+        | @tyVar' _ _ v => add v a s
+        | _ => None
+        end
+      | @tyApp _ _ _ va =>
+        match b with
+        | @tyApp _ _ _ vb =>
+          (fix go n n' (va : Vector.vector _ n) (vb : Vector.vector _ n') (s : Sub)
+           : option Sub :=
+             match va , vb with
+             | Vector.Vnil _ , Vector.Vnil _ => Some s
+             | Vector.Vcons a va , Vector.Vcons b vb =>
+               match type_unify a b s with
+               | Some s' => go _ _ va vb s'
+               | _ => None
+               end
+             | _ , _ => None
+             end) _ _ va vb s
+        | @tyVar' _ _ v => add v a s
+        | _ => None
+        end
+      | @tyProp _ => match b with
+                 | @tyProp _ => Some s
+                 | @tyVar' _ _ v => add v a s
+                 | _ => None
+                 end
+      | @tyVar' _ _ v =>
+        match b with
+        | @tyVar' _ _ v' => Some s
+        | _ => add v b s
+        end
+      end.
+
+  End with_symbols.
+
+End TypeLangUnify_mtyp.
+
+Export MirrorCore.Types.ModularTypesT.
+
+Definition kind : Set := TypeLang_mtyp.kind.
+Definition kindD : kind -> Type@{Ukind} := TypeLang_mtyp.kindD.
